steel/Zeta.Steel.Verifier.fsti
@@ -52,7 +52,23 @@ let verify_post_out_bytes (tsm:M.thread_state_model)
      array_pts_to out out_bytes1 `star`  //the out array contains out_bytes
      pure (Application.n_out_bytes tsm (M.verify_model tsm les) 0ul wrote out_bytes out_bytes1))
 
-
+[@@ __reduce__]
+let verify_post_success_pred
+  (tsm:M.thread_state_model)
+  (t:thread_state_t)
+  (log_bytes:bytes)
+  (out_bytes:bytes)
+  (out:A.array U8.t)
+  (aeh:AEH.aggregate_epoch_hashes)
+  (read wrote:U32.t)
+  : Seq.seq log_entry -> vprop
+  = fun log -> 
+    let tsm' = M.verify_model tsm log in
+    pure (parse_log_up_to log_bytes (U32.v read) == Some log) `star`
+    thread_state_inv t tsm' `star` //tsm' is the new state of the thread
+    TLM.tid_pts_to aeh.mlogs tsm'.thread_id full tsm'.processed_entries false `star` //my contributions are updated
+    verify_post_out_bytes tsm out_bytes wrote out log
+  
 let verify_post (tsm:M.thread_state_model)
                 (t:thread_state_t) //handle to the thread state
                 (log_bytes:bytes)
@@ -63,12 +79,7 @@ let verify_post (tsm:M.thread_state_model)
  : vprop
  = match res with
    | Verify_success read wrote ->
-     exists_ (fun log ->
-       let tsm' = M.verify_model tsm log in
-       pure (parse_log_up_to log_bytes (U32.v read) == Some log) `star`
-       thread_state_inv t tsm' `star` //tsm' is the new state of the thread
-       TLM.tid_pts_to aeh.mlogs tsm'.thread_id full tsm'.processed_entries false `star` //my contributions are updated
-       verify_post_out_bytes tsm out_bytes wrote out log)
+     exists_ (verify_post_success_pred tsm t log_bytes out_bytes out aeh read wrote)
    | _ ->
      some_failure t out aeh
        `star`
